updated some GDElemmas

backend/AllocproofEFF.v
@@ -1807,65 +1807,27 @@ Qed.
 Lemma GDE_lemma: genvs_domain_eq ge tge.
 Proof.
     unfold genvs_domain_eq, genv2blocks.
-    simpl; split; intros.
+    simpl; split; intros. 
      split; intros; destruct H as [id Hid].
-      rewrite <- symbols_preserved in Hid.
-      exists id; assumption.
+       rewrite <- symbols_preserved in Hid.
+       exists id; trivial.
      rewrite symbols_preserved in Hid.
-      exists id; assumption.
-     split; intros; destruct H as [id Hid].
-      rewrite <- varinfo_preserved in Hid.
-      exists id; assumption.
-     rewrite varinfo_preserved in Hid.
-      exists id; assumption.
-Qed.
-
-(*LENB: GFP as in selectionproofEFF*)
-Definition globalfunction_ptr_inject (j:meminj):=
-  forall b f, Genv.find_funct_ptr ge b = Some f -> 
-              j b = Some(b,0) /\ isGlobalBlock ge b = true.  
-
-Lemma restrict_preserves_globalfun_ptr: forall j X
-  (PG : globalfunction_ptr_inject j)
-  (Glob : forall b, isGlobalBlock ge b = true -> X b = true),
-globalfunction_ptr_inject (restrict j X).
-Proof. intros.
-  red; intros. 
-  destruct (PG _ _ H). split; trivial.
-  apply restrictI_Some; try eassumption.
-  apply (Glob _ H1).
-Qed.
-
-Lemma restrict_GFP_vis: forall mu
-  (GFP : globalfunction_ptr_inject (as_inj mu))
-  (Glob : forall b, isGlobalBlock ge b = true -> 
-                    frgnBlocksSrc mu b = true),
-  globalfunction_ptr_inject (restrict (as_inj mu) (vis mu)).
-Proof. intros.
-  unfold vis. 
-  eapply restrict_preserves_globalfun_ptr. eassumption.
-  intuition.
-Qed.
-
-(*From Cminorgenproof*)
-Remark val_inject_function_pointer:
-  forall v fd j tv,
-  Genv.find_funct ge v = Some fd ->
-  globalfunction_ptr_inject j ->
-  val_inject j v tv ->
-  tv = v.
-Proof.
-  intros. exploit Genv.find_funct_inv; eauto. intros [b EQ]. subst v.
-  inv H1.
-  rewrite Genv.find_funct_find_funct_ptr in H.
-  destruct (H0 _ _ H).
-  rewrite H1 in H4; inv H4.
-  rewrite Int.add_zero. trivial.
-Qed.
+       exists id; trivial.
+    split. intros. rewrite varinfo_preserved. intuition.
+    intros. split.
+      intros [f H].
+        apply function_ptr_translated in H. 
+        destruct H as [? [? _]]. 
+        eexists; eassumption.
+     intros [f H]. 
+         apply (@Genv.find_funct_ptr_rev_transf_partial
+           _ _ _ transf_fundef prog _ TRANSF) in H.
+         destruct H as [? [? _]]. eexists; eassumption.
+Qed.         
 
 Lemma find_function_translated:
   forall j ros rs fd ros' e e' ls
-  (GFP: globalfunction_ptr_inject j),
+  (GFP: globalfunction_ptr_inject ge j),
   RTL.find_function ge ros rs = Some fd ->
   add_equation_ros ros ros' e = Some e' ->
   satisf j rs ls e' ->
@@ -2234,7 +2196,7 @@ Definition MATCH mu c1 m1 c2 m2:Prop :=
   match_states (restrict (as_inj mu) (vis mu)) c1 m1 c2 m2 /\
   REACH_closed m1 (vis mu) /\
   meminj_preserves_globals ge (as_inj mu) /\
-  globalfunction_ptr_inject (as_inj mu) /\
+  globalfunction_ptr_inject ge (as_inj mu) /\
   (forall b, isGlobalBlock ge b = true -> frgnBlocksSrc mu b = true) /\
   sm_valid mu m1 m2 /\ SM_wd mu /\ Mem.inject (as_inj mu) m1 m2.
 
@@ -2469,11 +2431,9 @@ Lemma MATCH_initial: forall v
             (DomS b1 = true /\ DomT b2 = true))
       (RCH: forall b, REACH m2 
           (fun b' : block => isGlobalBlock tge b' || getBlocks vals2 b') b = true ->
-          DomT b = true)
-      (InitMem : exists m0 : mem, Genv.init_mem prog = Some m0 
-               /\ Ple (Mem.nextblock m0) (Mem.nextblock m1) 
-               /\ Ple (Mem.nextblock m0) (Mem.nextblock m2))   
+          DomT b = true) 
       (GDE: genvs_domain_eq ge tge)
+      (GFP: globalfunction_ptr_inject ge j)
       (HDomS: forall b : block, DomS b = true -> Mem.valid_block m1 b)
       (HDomT: forall b : block, DomT b = true -> Mem.valid_block m2 b),
 exists c2,
@@ -2625,18 +2585,11 @@ Proof. intros.
       assumption.
       apply BB.
       apply EE.
-    (*as in selectionprffEFF*)
-    (*globalfunctionptr*)
     rewrite initial_SM_as_inj.
-      red; intros. specialize (Genv.find_funct_ptr_not_fresh prog). intros.
-         destruct InitMem as [m0 [INIT_MEM [? ?]]].
-         specialize (H0 _ _ _ INIT_MEM H). 
-         destruct (valid_init_is_global _ R _ INIT_MEM _ H0) as [id Hid]. 
-           destruct PG as [PGa [PGb PGc]]. split. eapply PGa; eassumption.
-         unfold isGlobalBlock. 
-          apply orb_true_iff. left. apply genv2blocksBool_char1.
-            simpl. exists id; eassumption.
-    rewrite initial_SM_as_inj; assumption.
+    red; intros. 
+    destruct PG as [X [Y Z]].
+    solve[eapply GFP; eauto].
+    rewrite initial_SM_as_inj. assumption. 
 Qed.
 
 Lemma loc_result_locs_diff sig : locs_diff (map R (loc_result sig)).
@@ -3941,7 +3894,7 @@ induction CS;
         rewrite <- restrict_sm_all.
         eapply restrict_sm_preserves_globals; try eassumption.
           unfold vis. intuition.
-  assert (GFPR: globalfunction_ptr_inject (restrict (as_inj mu) (vis mu))). 
+  assert (GFPR: globalfunction_ptr_inject ge (restrict (as_inj mu) (vis mu))). 
             eapply restrict_GFP_vis; eassumption.
   destruct SP as [spb [spb' [B [B' Rsp]]]]; subst. inv B.
   destruct (restrictD_Some _ _ _ _ _ Rsp).
